Kami/PrimBram.v
@@ -29,7 +29,8 @@ Definition optionVal {ty dType} (ov: option (ty dType)):
 Definition liftSome {A} (a: A): option A :=
   Some a.
 
-Definition primBramName: string := "BRAM".
+Definition primBramName1: string := "BRAM1".
+Definition primBramName2: string := "BRAM2".
 
 Section PrimBram.
   Variables (bramName: string)
@@ -38,59 +39,88 @@ Section PrimBram.
 
   Local Notation "^ s" := (bramName -- s) (at level 0).
 
-  Definition bramReadValT (ty: Kind -> Type) := option (ty dType).
-  Definition bramReadValK ty := @NativeKind (bramReadValT ty) None.
-  Definition bramReadVal ty :=
-    (^"rss" :: (@NativeConst (bramReadValT ty) None None))%struct.
+  Definition bramReadAddrT (ty: Kind -> Type) := option (ty (Bit addrSize)).
+  Definition bramReadAddrK ty := @NativeKind (bramReadAddrT ty) None.
 
   Definition BramRq :=
-    STRUCT {
-        "write" :: Bool;
-        "addr" :: Bit addrSize;
-        "datain" :: dType
-      }.
-  
+    STRUCT { "write" :: Bool;
+             "addr" :: Bit addrSize;
+             "datain" :: dType }.
+
   Definition bramPutRq: forall ty (rq: ty (Struct BramRq)), ActionT ty Void :=
     fun ty rq =>
-      (Read bram <- ^"bram";
-       If #rq!BramRq@."write" then
-         LET writev <- #rq!BramRq@."datain";
-         Write ^"bram" <- #bram@[#rq!BramRq@."addr" <- #writev];
-         Retv
-       else
-         ReadN readVal: bramReadValK ty <- ^"readVal";
-         Assert $$(isNoneB readVal);
-         LET readv: dType <- #bram@[#rq!BramRq@."addr"];
-         Write ^"readVal" <- Var _ (bramReadValK ty) (liftSome readv);
-         Retv;
-       Retv)%kami_action.
+      (If #rq!BramRq@."write"
+       then (LET writev <- #rq!BramRq@."datain";
+            Read bram <- ^"bram";
+            Write ^"bram" <- #bram@[#rq!BramRq@."addr" <- #writev];
+            Retv)
+       else (ReadN readAddr: bramReadAddrK ty <- ^"readAddr";
+            Assert $$(isNoneB readAddr);
+            LET raddr <- #rq!BramRq@."addr";
+            Write ^"readAddr" <- Var _ (bramReadAddrK ty) (liftSome raddr);
+            Retv);
+      Retv)%kami_action.
 
-  Definition bramGetRs: forall ty (_: ty Void), ActionT ty dType :=
+  Definition bramReadRs: forall ty (_: ty Void), ActionT ty dType :=
     fun ty _ =>
-      (ReadN readVal: bramReadValK ty <- ^"readVal";
-       Assert $$(isSomeB readVal);
-       Write ^"readVal" <- (Var _ (bramReadValK ty) None);
-       Ret (optionVal readVal)%kami_action)%kami_action.
-  
+      (ReadN oreadAddr: bramReadAddrK ty <- ^"readAddr";
+      Assert $$(isSomeB oreadAddr);
+      Write ^"readAddr" <- (Var _ (bramReadAddrK ty) None);
+      Read bram: Vector dType addrSize <- ^"bram";
+      LET reada <- optionVal oreadAddr;
+      LET readv: dType <- #bram@[#reada];
+      Ret #readv)%kami_action.
+
   Definition bram1: Modules :=
     PrimMod
-      {| pm_name := primBramName;
+      {| pm_name := primBramName1;
          pm_regInits :=
            [(^"bram" :: (RegInitDefault (SyntaxKind (Vector dType addrSize))))%struct;
-              (^"readVal" :: (RegInitCustom (existT ConstFullT (bramReadValK type)
-                                                    (NativeConst None None))))%struct];
+           (^"readAddr" :: (RegInitCustom (existT ConstFullT (bramReadAddrK type)
+                                                  (NativeConst None None))))%struct];
          pm_rules := nil;
          pm_methods :=
            [(^"putRq" :: (existT _ {| arg:= _; ret:= _ |} bramPutRq))%struct;
-              (^"getRs" :: (existT _ {| arg:= _; ret:= _ |} bramGetRs))%struct]
+           (^"readRs" :: (existT _ {| arg:= _; ret:= _ |} bramReadRs))%struct]
+      |}.
+
+  Definition bramReadRq: forall ty (addr: ty (Bit addrSize)), ActionT ty Void :=
+    fun ty addr =>
+      (ReadN readAddr: bramReadAddrK ty <- ^"readAddr";
+      Assert $$(isNoneB readAddr);
+      Write ^"readAddr" <- Var _ (bramReadAddrK ty) (liftSome addr);
+      Retv)%kami_action.
+
+  Definition BramWriteRq :=
+    STRUCT { "addr" :: Bit addrSize; "datain" :: dType }.
+
+  Definition bramWriteRq: forall ty (rq: ty (Struct BramWriteRq)), ActionT ty Void :=
+    fun ty rq =>
+      (LET writev <- #rq!BramWriteRq@."datain";
+      Read bram <- ^"bram";
+      Write ^"bram" <- #bram@[#rq!BramWriteRq@."addr" <- #writev];
+      Retv)%kami_action.
+
+  Definition bram2: Modules :=
+    PrimMod
+      {| pm_name := primBramName1;
+         pm_regInits :=
+           [(^"bram" :: (RegInitDefault (SyntaxKind (Vector dType addrSize))))%struct;
+           (^"readAddr" :: (RegInitCustom (existT ConstFullT (bramReadAddrK type)
+                                                  (NativeConst None None))))%struct];
+         pm_rules := nil;
+         pm_methods :=
+           [(^"rdReq" :: (existT _ {| arg:= _; ret:= _ |} bramReadRq))%struct;
+           (^"wrReq" :: (existT _ {| arg:= _; ret:= _ |} bramWriteRq))%struct;
+           (^"readRs" :: (existT _ {| arg:= _; ret:= _ |} bramReadRs))%struct]
       |}.
 
 End PrimBram.
 
-Hint Unfold bram1 : ModuleDefs.
-Hint Unfold primBramName
-     bramReadValT bramReadValK bramReadVal
-     BramRq bramPutRq bramGetRs: MethDefs.
+Hint Unfold bram1 bram2: ModuleDefs.
+Hint Unfold primBramName1 primBramName2
+     bramReadAddrT bramReadAddrK
+     BramRq bramPutRq bramReadRs bramReadRq BramWriteRq bramWriteRq: MethDefs.
 
 Section Facts.
   Variables (bramName: string)
@@ -111,8 +141,21 @@ Section Facts.
   Qed.
   Hint Resolve bram1_ValidRegs.
 
+  Lemma bram2_ModEquiv:
+    ModPhoasWf (bram2 bramName addrSize dType).
+  Proof.
+    kequiv.
+  Qed.
+  Hint Resolve bram2_ModEquiv.
+
+  Lemma bram2_ValidRegs:
+    ModRegsWf (bram2 bramName addrSize dType).
+  Proof.
+    kvr.
+  Qed.
+  Hint Resolve bram2_ValidRegs.
+
 End Facts.
 
-Hint Resolve bram1_ModEquiv.
-Hint Resolve bram1_ValidRegs.
-
+Hint Resolve bram1_ModEquiv bram2_ModEquiv.
+Hint Resolve bram1_ValidRegs bram2_ValidRegs.
